interpreter.v
@@ -1,6 +1,8 @@
 (* Copyright (c) 2012-2014, Robbert Krebbers. *)
 (* This file is distributed under the terms of the BSD license. *)
+Require Import String.
 Require Export executable frontend natural_type_environment two_complement.
+Local Open Scope string_scope.
 
 Section interpreter.
 Context (be : bool) (Csz : nat).
@@ -13,10 +15,13 @@ Existing Instance ptr_env.
 
 Definition interpreter (Θ : list (N * decl Ti))
     (f : funname) (vs : list (val Ti)) :
-    option (stream (listset (state Ti) * listset (state Ti))) :=
+    string + stream (listset (state Ti) * listset (state Ti)) :=
   '(Γ,Γf,δ,m) ← to_envs Θ;
-  '(σs,_) ← Γf !! f;
-  σs' ← mapM (type_check (Γ,m)) vs;
-  guard (σs' = (σs : list (type Ti)));
-  Some (csteps_exec hash Γ δ {[ initial_state m f vs ]}).
+  '(σs,_) ← error_of_option (Γf !! f)
+    "interpreter called with function that does not exists";
+  σs' ← error_of_option (mapM (type_check (Γ,m)) vs)
+    "interpreter called with values that cannot be typed";
+  guard (σs' = (σs : list (type Ti)))
+    with "interpreter called with values of incorrect type";
+  inr (csteps_exec hash Γ δ {[ initial_state m f vs ]}).
 End interpreter.
